new_example/timestamp_proof.v
@@ -13,25 +13,14 @@ Module TimeStamp_Proof.
     Program Instance : IsPkgInit main :=
         ltac2:(build_pkg_init ()).
 
-    Record C :=
-      mkC {
-          hour: u32;
-          minute: u32;
-          second: u32;
-      }.
-
-    (* Definition has_encoding (encoded:list u8) (args:main.TimeStamp.t) : Prop := *)
-    (*   encoded = (u32_le args.(main.TimeStamp.hour')) ++ (u32_le args.(main.TimeStamp.minute')) *)
-    (*               ++ (u32_le args.(main.TimeStamp.second')). *)
-
-    Definition has_encoding' (encoded:list u8) (args:C) : Prop :=
-      encoded = (u32_le args.(hour)) ++ (u32_le args.(minute))
-                  ++ (u32_le args.(second)).
+    Definition C := main.TimeStamp.t.
+    
+    Definition has_encoding (encoded:list u8) (args:C) : Prop :=
+      encoded = (u32_le args.(main.TimeStamp.hour')) ++ (u32_le args.(main.TimeStamp.minute'))
+                  ++ (u32_le args.(main.TimeStamp.second')).
 
     Definition own (v:main.TimeStamp.t) (c:C) (dq:dfrac) : iProp Σ :=
-      ⌜ v.(main.TimeStamp.hour') = c.(hour) ⌝ ∗
-      ⌜ v.(main.TimeStamp.minute') = c.(minute) ⌝ ∗
-      ⌜ v.(main.TimeStamp.second') = c.(second) ⌝. 
+      ⌜ v = c ⌝.
 
     Lemma wp_Encode (args__t : main.TimeStamp.t) (args__c:C) (pre_sl : slice.t) (prefix : list u8) (dq : dfrac):
       {{{
@@ -43,7 +32,7 @@ Module TimeStamp_Proof.
         main @ "MarshalTimeStamp" #pre_sl #args__t
       {{{
             enc enc_sl, RET #enc_sl;
-            ⌜ has_encoding' enc args__c ⌝ ∗
+            ⌜ has_encoding enc args__c ⌝ ∗
             own_slice enc_sl (DfracOwn 1) (prefix ++ enc) ∗
             own_slice_cap w8 enc_sl ∗
             own args__t args__c dq
@@ -51,7 +40,7 @@ Module TimeStamp_Proof.
 
     Proof. 
         wp_start as "(Hown & Hsl & Hcap)". wp_auto.
-        iDestruct "Hown" as "(%Hhour & %Hminute & %Hsecond)".
+        iDestruct "Hown" as "%Hown".
 
         wp_apply (wp_WriteInt32 with "[$Hsl $Hcap]").
         iIntros (?) "[Hsl Hcap]". wp_auto.
@@ -63,8 +52,7 @@ Module TimeStamp_Proof.
         iIntros (?) "[Hsl Hcap]". wp_auto.
 
         iApply "HΦ". rewrite -?app_assoc. iFrame.
-        iPureIntro. unfold has_encoding'.
-        rewrite Hhour. rewrite Hminute. rewrite Hsecond.
+        iPureIntro. unfold has_encoding. subst.
         done.
     Qed.
 
@@ -72,7 +60,7 @@ Module TimeStamp_Proof.
       {{{
             is_pkg_init main ∗
             own_slice enc_sl dq (enc ++ suffix) ∗
-            ⌜ has_encoding' enc args__c ⌝
+            ⌜ has_encoding enc args__c ⌝
       }}}
         main @ "UnmarshalTimeStamp" #enc_sl
       {{{
@@ -83,7 +71,7 @@ Module TimeStamp_Proof.
         
     Proof.
       wp_start as "[Hsl %Henc]". wp_auto.
-      unfold has_encoding' in Henc. rewrite Henc. rewrite -?app_assoc.
+      unfold has_encoding in Henc. rewrite Henc. rewrite -?app_assoc.
 
       wp_apply (wp_ReadInt32 with "[$Hsl]").
       iIntros (?) "Hsl". wp_auto.
@@ -94,12 +82,13 @@ Module TimeStamp_Proof.
       wp_apply (wp_ReadInt32 with "[$Hsl]").
       iIntros (?) "Hsl". wp_auto.
 
-      (* replace {| *)
-      (*  main.TimeStamp.hour' := args__c.(hour); *)
-      (*  main.TimeStamp.minute' := args__c.(minute); *)
-      (*  main.TimeStamp.second' := args__c.(second) *)
-      (*   |} with args__t; last (destruct args__t; reflexivity). *)
-      iApply "HΦ". iFrame. done.
+      iApply "HΦ". iFrame.
+      replace {|
+       main.TimeStamp.hour' := args__c.(main.TimeStamp.hour');
+       main.TimeStamp.minute' := args__c.(main.TimeStamp.minute');
+       main.TimeStamp.second' := args__c.(main.TimeStamp.second')
+        |} with args__c; last (destruct args__c; reflexivity).
+      done.
     Qed.
   End TimeStamp_Proof.
 End TimeStamp_Proof.
