Makefile
@@ -2,13 +2,13 @@ SRC_DIRS := 'perennial' 'new_example' 'testdata/out'
 ALL_VFILES := $(shell find $(SRC_DIRS) -not -path "perennial/external/coqutil/etc/coq-scripts/*" -name "*.v")
 PROJ_VFILES := $(shell find 'new_example' -name "*.v")
 
-# extract any global arguments for Coq from _CoqProject
-COQPROJECT_ARGS := $(shell sed -E -e '/^\#/d' -e "s/'([^']*)'/\1/g" -e 's/-arg //g' _CoqProject)
+# extract any global arguments for Rocq from _RocqProject
+ROCQ_PROJECT_ARGS := $(shell sed -E -e '/^\#/d' -e "s/'([^']*)'/\1/g" -e 's/-arg //g' _RocqProject)
 
 # user configurable
 Q:=@
-COQ_ARGS := -noglob
-COQC := coqc
+ROCQ_ARGS := -noglob
+ROCQ_C := rocq compile
 
 default: vo
 
@@ -18,33 +18,33 @@ vok: $(PROJ_VFILES:.v=.vok)
 
 all: vo
 
-.coqdeps.d: $(ALL_VFILES) _CoqProject
-	@echo "COQDEP $@"
-	$(Q)coqdep -vos -f _CoqProject $(ALL_VFILES) > $@
+.rocqdeps.d: $(ALL_VFILES) _RocqProject
+	@echo "ROCQ DEP $@"
+	$(Q)rocq dep -vos -f _RocqProject $(ALL_VFILES) > $@
 
 # do not try to build dependencies if cleaning
 ifeq ($(filter clean,$(MAKECMDGOALS)),)
--include .coqdeps.d
+-include .rocqdeps.d
 endif
 
-%.vo: %.v _CoqProject | .coqdeps.d
-	@echo "COQC $<"
-	$(Q)$(COQC) $(COQPROJECT_ARGS) $(COQ_ARGS) -o $@ $<
+%.vo: %.v _RocqProject | .rocqdeps.d
+	@echo "ROCQ COMPILE $<"
+	$(Q)$(ROCQ_C) $(ROCQ_PROJECT_ARGS) $(ROCQ_ARGS) -o $@ $<
 
-%.vos: %.v _CoqProject | .coqdeps.d
-	@echo "COQC -vos $<"
-	$(Q)$(COQC) $(COQPROJECT_ARGS) -vos $(COQ_ARGS) $< -o $@
+%.vos: %.v _RocqProject | .rocqdeps.d
+	@echo "ROCQ COMPILE -vos $<"
+	$(Q)$(ROCQ_C) $(ROCQ_PROJECT_ARGS) -vos $(ROCQ_ARGS) $< -o $@
 
-%.vok: %.v _CoqProject | .coqdeps.d
-	@echo "COQC -vok $<"
-	$(Q)$(COQC) $(COQPROJECT_ARGS) -vok $(COQ_ARGS) $< -o $@
+%.vok: %.v _RocqProject | .rocqdeps.d
+	@echo "ROCQ COMPILE -vok $<"
+	$(Q)$(ROCQ) $(ROCQ_PROJECT_ARGS) -vok $(ROCQ_ARGS) $< -o $@
 
 clean:
 	@echo "CLEAN vo glob aux"
 	$(Q)find $(SRC_DIRS) \( -name "*.vo" -o -name "*.vo[sk]" \
 		-o -name ".*.aux" -o -name ".*.cache" -name "*.glob" \) -delete
 	$(Q)rm -f .timing.sqlite3
-	rm -f .coqdeps.d
+	rm -f .rocqdeps.d
 
 .PHONY: default
 .DELETE_ON_ERROR:
